Some helper definitions and lemma statements
We need to operate on state merges (and their unpartializations) of
pairs of mergeable states. Some auxiliary results will smoothen the
structure of coming proofs.

Intermediate/PS.v
@@ -882,6 +882,12 @@ Definition mergeable_states_pc (s s' : state) : Pointer.t :=
     | _, _ => (Component.main, 0, 0%Z)
   end.
 
+Definition mergeable_states_state (s s' : state) : state :=
+  PS.PC (mergeable_states_stack s s',
+         mergeable_states_memory s s',
+         mergeable_states_regs s s',
+         mergeable_states_pc s s').
+
 (* transition system *)
 
 Inductive initial_state (p: program) (ctx: Program.interface) : state -> Prop :=
