Intermediate/Composition.v
@@ -3600,12 +3600,40 @@ Section MultiSemantics.
         eapply (@execution_invariant_to_linking _ _ _ _ _ Hlinkable'); assumption.
   Qed.
 
+  (* RB: TODO: Add side conditions (well-formed programs, linkable interfaces,
+     etc. *)
+  Lemma mergeable_states_merge :
+    forall s s',
+      PS.mergeable_states (prog_interface c) (prog_interface p) s s' ->
+      PS.merge_partial_states s s' =
+      PS.mergeable_states_state s s'.
+  Admitted. (* Grade 2. *)
+
+  (* A special case of a more general property on [PS.partial_state emptym] that
+     would relate a CS state to its injection to a PS state. *)
+  Lemma mergeable_states_partial_state_emptym :
+    forall s s',
+      PS.mergeable_states (prog_interface c) (prog_interface p) s s' ->
+      PS.partial_state emptym
+                       (PS.unpartialize (PS.merge_partial_states s s'))
+                       (PS.merge_partial_states s s').
+  Admitted. (* Grade 1. *)
+
+  Lemma mergeable_states_step_CS : forall s1 s1' s2 s2' t,
+    PS.mergeable_states (prog_interface c) (prog_interface p) s1 s1' ->
+    PS.step p (prog_interface c) (prepare_global_env p) s1 t s2 ->
+    PS.step c (prog_interface p) (prepare_global_env c) s1' t s2'->
+    CS.step (prepare_global_env (program_link p c))
+            (PS.unpartialize (PS.merge_partial_states s1 s1')) t
+            (PS.unpartialize (PS.merge_partial_states s2 s2')).
+  Admitted.
+
   (* RB: TODO: This result very likely belongs in PS. I am reusing the hypotheses
      in this section, but these should be pared down. *)
   Lemma mergeable_states_step : forall s1 s1' s2 s2' t,
     PS.mergeable_states (prog_interface c) (prog_interface p) s1 s1' ->
     PS.step p (prog_interface c) (prepare_global_env p) s1 t s2 ->
-    PS.step c (prog_interface p) (prepare_global_env c) s1' t s2' ->
+    PS.step c (prog_interface p) (prepare_global_env c) s1' t s2'->
     PS.step (program_link p c) emptym (prepare_global_env (program_link p c))
             (PS.merge_partial_states s1 s1') t
             (PS.merge_partial_states s2 s2').
